add trait ready body callee evidence

rocq/theories/TypeSystem/TypeSafetyDirectCallEvidenceFacts.v
@@ -797,6 +797,50 @@ Definition direct_call_callee_body_root_evidence (env : global_env) : Prop :=
     callee_body_root_ready_at env fcall
       (call_param_root_env (fn_params fcall) arg_roots R_args).
 
+Definition direct_call_callee_body_root_evidence_at
+    (env : global_env) (fname : ident) : Prop :=
+  forall (Ω : outlives_ctx) (n : nat) R Σ Σ_args R_args arg_roots
+      args fdef fcall (σ : list lifetime) s s_args vs used',
+    In fdef (env_fns env) ->
+    fn_name fdef = fname ->
+    fn_captures fdef = [] ->
+    typed_args_roots env Ω n R Σ args
+      (apply_lt_params σ (fn_params fdef)) Σ_args R_args arg_roots ->
+    eval_args env s args s_args vs ->
+    provenance_ready_args args ->
+    store_typed env s Σ ->
+    store_roots_within R s ->
+    store_no_shadow s ->
+    root_env_no_shadow R ->
+    root_env_store_roots_named R s ->
+    root_env_store_keys_named R s ->
+    alpha_rename_fn_def (store_names s_args) fdef = (fcall, used') ->
+    callee_body_root_ready_at env fcall
+      (call_param_root_env (fn_params fcall) arg_roots R_args).
+
+Definition direct_call_callee_body_root_ready_body_evidence_at
+    (env : global_env) (fname : ident) : Prop :=
+  forall (Ω : outlives_ctx) (n : nat) R Σ Σ_args R_args arg_roots
+      args fdef fcall (σ : list lifetime) s s_args vs used',
+    In fdef (env_fns env) ->
+    fn_name fdef = fname ->
+    fn_captures fdef = [] ->
+    typed_args_roots env Ω n R Σ args
+      (apply_lt_params σ (fn_params fdef)) Σ_args R_args arg_roots ->
+    eval_args env s args s_args vs ->
+    provenance_ready_args args ->
+    store_typed env s Σ ->
+    store_roots_within R s ->
+    store_no_shadow s ->
+    root_env_no_shadow R ->
+    root_env_store_roots_named R s ->
+    root_env_store_keys_named R s ->
+    alpha_rename_fn_def (store_names s_args) fdef = (fcall, used') ->
+    callee_body_root_synthetic_direct_call_ready_at env fcall
+      (call_param_root_env (fn_params fcall) arg_roots R_args) \/
+    callee_body_root_ready_at env fcall
+      (call_param_root_env (fn_params fcall) arg_roots R_args).
+
 Definition direct_call_callee_body_root_direct_call_ready_summary_bridge
     (env : global_env) : Prop :=
   env_fns_root_direct_call_ready_summary_evidence env ->
@@ -953,6 +997,51 @@ Definition direct_call_callee_body_root_synthetic_direct_call_ready_evidence_at
     alpha_rename_fn_def (store_names s_args) fdef = (fcall, used') ->
     callee_body_root_synthetic_direct_call_ready_at env fcall
       (call_param_root_env (fn_params fcall) arg_roots R_args).
+
+Lemma direct_call_callee_body_root_evidence_at_of_evidence :
+  forall env fname,
+    direct_call_callee_body_root_evidence env ->
+    direct_call_callee_body_root_evidence_at env fname.
+Proof.
+  intros env fname Hevidence Ω n R Σ Σ_args R_args arg_roots args
+    fdef fcall σ s s_args vs used' Hin Hname Hcaps Htyped_args
+    Heval_args Hprov_args Hstore Hroots Hshadow Hrn Hnamed Hkeys Hrename.
+  eapply Hevidence; eassumption.
+Qed.
+
+Lemma direct_call_callee_body_root_ready_body_evidence_at_of_synthetic :
+  forall env fname,
+    direct_call_callee_body_root_synthetic_direct_call_ready_evidence_at
+      env fname ->
+    direct_call_callee_body_root_ready_body_evidence_at env fname.
+Proof.
+  intros env fname Hevidence Ω n R Σ Σ_args R_args arg_roots args
+    fdef fcall σ s s_args vs used' Hin Hname Hcaps Htyped_args
+    Heval_args Hprov_args Hstore Hroots Hshadow Hrn Hnamed Hkeys Hrename.
+  left. eapply Hevidence; eassumption.
+Qed.
+
+Lemma direct_call_callee_body_root_ready_body_evidence_at_of_ordinary :
+  forall env fname,
+    direct_call_callee_body_root_evidence_at env fname ->
+    direct_call_callee_body_root_ready_body_evidence_at env fname.
+Proof.
+  intros env fname Hevidence Ω n R Σ Σ_args R_args arg_roots args
+    fdef fcall σ s s_args vs used' Hin Hname Hcaps Htyped_args
+    Heval_args Hprov_args Hstore Hroots Hshadow Hrn Hnamed Hkeys Hrename.
+  right. eapply Hevidence; eassumption.
+Qed.
+
+Lemma direct_call_callee_body_root_ready_body_evidence_at_of_evidence :
+  forall env fname,
+    direct_call_callee_body_root_evidence env ->
+    direct_call_callee_body_root_ready_body_evidence_at env fname.
+Proof.
+  intros env fname Hevidence.
+  eapply direct_call_callee_body_root_ready_body_evidence_at_of_ordinary.
+  eapply direct_call_callee_body_root_evidence_at_of_evidence.
+  exact Hevidence.
+Qed.
 
 Lemma direct_call_callee_body_root_evidence_of_summary_bridge :
   forall env,
